stdlib/lampe/Stdlib/Ops/Bit.lean
@@ -4,3 +4,665 @@ import Lampe
 namespace Lampe.Stdlib.Ops.Bit
 
 open «std-1.0.0-beta.12»
+
+set_option Lampe.pp.Expr false
+set_option Lampe.pp.STHoare false
+
+/-- A shorthand for a call to the `std::ops::bit::Not::not` method. -/
+@[reducible]
+def not {p}
+    (generics : HList Kind.denote «std-1.0.0-beta.12::ops::bit::Not».«#genericKinds»)
+    (Self : Tp)
+    (associatedTypes : HList Kind.denote «std-1.0.0-beta.12::ops::bit::Not».«#associatedTypesKinds»)
+    (fnGenerics : HList Kind.denote «std-1.0.0-beta.12::ops::bit::Not».not.«#genericKinds»)
+  : HList (Tp.denote p)
+      («std-1.0.0-beta.12::ops::bit::Not».not.«#inputs» generics Self associatedTypes fnGenerics)
+  → Expr (Tp.denote p)
+      («std-1.0.0-beta.12::ops::bit::Not».not.«#output» generics Self associatedTypes fnGenerics) :=
+  «std-1.0.0-beta.12::ops::bit::Not».not generics Self associatedTypes fnGenerics
+
+set_option maxRecDepth 1300 in
+theorem bool_not_spec {p a}
+  : STHoare p env ⟦⟧
+    (not h![] .bool h![] h![] h![a])
+    (fun r => r = !a) := by
+  resolve_trait
+  steps
+  simp_all
+  exact ()
+
+set_option maxRecDepth 1300 in
+theorem u128_not_spec {p a}
+  : STHoare p env ⟦⟧
+    (not h![] (.u 128) h![] h![] h![a])
+    (fun r => r = a.not) := by
+  resolve_trait
+  steps
+  simp_all
+
+set_option maxRecDepth 1300 in
+theorem u64_not_spec {p a}
+  : STHoare p env ⟦⟧
+    (not h![] (.u 64) h![] h![] h![a])
+    (fun r => r = a.not) := by
+  resolve_trait
+  steps
+  simp_all
+
+set_option maxRecDepth 1300 in
+theorem u32_not_spec {p a}
+  : STHoare p env ⟦⟧
+    (not h![] (.u 32) h![] h![] h![a])
+    (fun r => r = a.not) := by
+  resolve_trait
+  steps
+  simp_all
+
+set_option maxRecDepth 1300 in
+theorem u16_not_spec {p a}
+  : STHoare p env ⟦⟧
+    (not h![] (.u 16) h![] h![] h![a])
+    (fun r => r = a.not) := by
+  resolve_trait
+  steps
+  simp_all
+
+set_option maxRecDepth 1300 in
+theorem u8_not_spec {p a}
+  : STHoare p env ⟦⟧
+    (not h![] (.u 8) h![] h![] h![a])
+    (fun r => r = a.not) := by
+  resolve_trait
+  steps
+  simp_all
+
+set_option maxRecDepth 1350 in
+theorem u1_not_spec {p a}
+  : STHoare p env ⟦⟧
+    (not h![] (.u 1) h![] h![] h![a])
+    (fun r => r = a.not) := by
+  resolve_trait
+  steps
+  simp_all
+
+set_option maxRecDepth 1350 in
+theorem i8_not_spec {p a}
+  : STHoare p env ⟦⟧
+    (not h![] (.i 8) h![] h![] h![a])
+    (fun r => r = a.not) := by
+  resolve_trait
+  steps
+  simp_all
+
+set_option maxRecDepth 1350 in
+theorem i16_not_spec {p a}
+  : STHoare p env ⟦⟧
+    (not h![] (.i 16) h![] h![] h![a])
+    (fun r => r = a.not) := by
+  resolve_trait
+  steps
+  simp_all
+
+set_option maxRecDepth 1350 in
+theorem i32_not_spec {p a}
+  : STHoare p env ⟦⟧
+    (not h![] (.i 32) h![] h![] h![a])
+    (fun r => r = a.not) := by
+  resolve_trait
+  steps
+  simp_all
+
+set_option maxRecDepth 1350 in
+theorem i64_not_spec {p a}
+  : STHoare p env ⟦⟧
+    (not h![] (.i 64) h![] h![] h![a])
+    (fun r => r = a.not) := by
+  resolve_trait
+  steps
+  simp_all
+
+/-- A shorthand for a call to the `std::ops::bit::BitOr::bitor` method. -/
+@[reducible]
+def bitOr {p}
+    (generics : HList Kind.denote «std-1.0.0-beta.12::ops::bit::BitOr».«#genericKinds»)
+    (Self : Tp)
+    (associatedTypes : HList Kind.denote «std-1.0.0-beta.12::ops::bit::BitOr».«#associatedTypesKinds»)
+    (fnGenerics : HList Kind.denote «std-1.0.0-beta.12::ops::bit::BitOr».bitor.«#genericKinds»)
+  : HList (Tp.denote p)
+      («std-1.0.0-beta.12::ops::bit::BitOr».bitor.«#inputs» generics Self associatedTypes fnGenerics)
+  → Expr (Tp.denote p)
+      («std-1.0.0-beta.12::ops::bit::BitOr».bitor.«#output» generics Self associatedTypes fnGenerics) :=
+  «std-1.0.0-beta.12::ops::bit::BitOr».bitor generics Self associatedTypes fnGenerics
+
+set_option maxRecDepth 1350 in
+theorem bool_bit_or_spec {p a b}
+  : STHoare p env ⟦⟧
+    (bitOr h![] .bool h![] h![] h![a, b])
+    (fun r => r = a.or b) := by
+  resolve_trait
+  steps
+  simp_all
+  exact ()
+
+set_option maxRecDepth 1350 in
+theorem u128_bit_or_spec {p a b}
+  : STHoare p env ⟦⟧
+    (bitOr h![] (.u 128) h![] h![] h![a, b])
+    (fun r => r = a.or b) := by
+  resolve_trait
+  steps
+  simp_all
+
+set_option maxRecDepth 1350 in
+theorem u64_bit_or_spec {p a b}
+  : STHoare p env ⟦⟧
+    (bitOr h![] (.u 64) h![] h![] h![a, b])
+    (fun r => r = a.or b) := by
+  resolve_trait
+  steps
+  simp_all
+
+set_option maxRecDepth 1350 in
+theorem u32_bit_or_spec {p a b}
+  : STHoare p env ⟦⟧
+    (bitOr h![] (.u 32) h![] h![] h![a, b])
+    (fun r => r = a.or b) := by
+  resolve_trait
+  steps
+  simp_all
+
+set_option maxRecDepth 1350 in
+theorem u16_bit_or_spec {p a b}
+  : STHoare p env ⟦⟧
+    (bitOr h![] (.u 16) h![] h![] h![a, b])
+    (fun r => r = a.or b) := by
+  resolve_trait
+  steps
+  simp_all
+
+set_option maxRecDepth 1350 in
+theorem u8_bit_or_spec {p a b}
+  : STHoare p env ⟦⟧
+    (bitOr h![] (.u 8) h![] h![] h![a, b])
+    (fun r => r = a.or b) := by
+  resolve_trait
+  steps
+  simp_all
+
+set_option maxRecDepth 1350 in
+theorem u1_bit_or_spec {p a b}
+  : STHoare p env ⟦⟧
+    (bitOr h![] (.u 1) h![] h![] h![a, b])
+    (fun r => r = a.or b) := by
+  resolve_trait
+  steps
+  simp_all
+
+set_option maxRecDepth 1350 in
+theorem i8_bit_or_spec {p a b}
+  : STHoare p env ⟦⟧
+    (bitOr h![] (.i 8) h![] h![] h![a, b])
+    (fun r => r = a.or b) := by
+  resolve_trait
+  steps
+  simp_all
+
+set_option maxRecDepth 1350 in
+theorem i16_bit_or_spec {p a b}
+  : STHoare p env ⟦⟧
+    (bitOr h![] (.i 16) h![] h![] h![a, b])
+    (fun r => r = a.or b) := by
+  resolve_trait
+  steps
+  simp_all
+
+set_option maxRecDepth 1350 in
+theorem i32_bit_or_spec {p a b}
+  : STHoare p env ⟦⟧
+    (bitOr h![] (.i 32) h![] h![] h![a, b])
+    (fun r => r = a.or b) := by
+  resolve_trait
+  steps
+  simp_all
+
+set_option maxRecDepth 1350 in
+theorem i64_bit_or_spec {p a b}
+  : STHoare p env ⟦⟧
+    (bitOr h![] (.i 64) h![] h![] h![a, b])
+    (fun r => r = a.or b) := by
+  resolve_trait
+  steps
+  simp_all
+
+/-- A shorthand for a call to the `std::ops::bit::BitOr::bitand` method. -/
+@[reducible]
+def bitAnd {p}
+    (generics : HList Kind.denote «std-1.0.0-beta.12::ops::bit::BitAnd».«#genericKinds»)
+    (Self : Tp)
+    (associatedTypes : HList Kind.denote «std-1.0.0-beta.12::ops::bit::BitAnd».«#associatedTypesKinds»)
+    (fnGenerics : HList Kind.denote «std-1.0.0-beta.12::ops::bit::BitAnd».bitand.«#genericKinds»)
+  : HList (Tp.denote p)
+      («std-1.0.0-beta.12::ops::bit::BitAnd».bitand.«#inputs» generics Self associatedTypes fnGenerics)
+  → Expr (Tp.denote p)
+      («std-1.0.0-beta.12::ops::bit::BitAnd».bitand.«#output» generics Self associatedTypes fnGenerics) :=
+  «std-1.0.0-beta.12::ops::bit::BitAnd».bitand generics Self associatedTypes fnGenerics
+
+set_option maxRecDepth 1350 in
+theorem bool_bit_and_spec {p a b}
+  : STHoare p env ⟦⟧
+    (bitAnd h![] .bool h![] h![] h![a, b])
+    (fun r => r = a.and b) := by
+  resolve_trait
+  steps
+  simp_all
+  exact ()
+
+set_option maxRecDepth 1400 in
+theorem u128_bit_and_spec {p a b}
+  : STHoare p env ⟦⟧
+    (bitAnd h![] (.u 128) h![] h![] h![a, b])
+    (fun r => r = a.and b) := by
+  resolve_trait
+  steps
+  simp_all
+
+set_option maxRecDepth 1400 in
+theorem u64_bit_and_spec {p a b}
+  : STHoare p env ⟦⟧
+    (bitAnd h![] (.u 64) h![] h![] h![a, b])
+    (fun r => r = a.and b) := by
+  resolve_trait
+  steps
+  simp_all
+
+set_option maxRecDepth 1400 in
+theorem u32_bit_and_spec {p a b}
+  : STHoare p env ⟦⟧
+    (bitAnd h![] (.u 32) h![] h![] h![a, b])
+    (fun r => r = a.and b) := by
+  resolve_trait
+  steps
+  simp_all
+
+set_option maxRecDepth 1400 in
+theorem u16_bit_and_spec {p a b}
+  : STHoare p env ⟦⟧
+    (bitAnd h![] (.u 16) h![] h![] h![a, b])
+    (fun r => r = a.and b) := by
+  resolve_trait
+  steps
+  simp_all
+
+set_option maxRecDepth 1400 in
+theorem u8_bit_and_spec {p a b}
+  : STHoare p env ⟦⟧
+    (bitAnd h![] (.u 8) h![] h![] h![a, b])
+    (fun r => r = a.and b) := by
+  resolve_trait
+  steps
+  simp_all
+
+set_option maxRecDepth 1400 in
+theorem u1_bit_and_spec {p a b}
+  : STHoare p env ⟦⟧
+    (bitAnd h![] (.u 1) h![] h![] h![a, b])
+    (fun r => r = a.and b) := by
+  resolve_trait
+  steps
+  simp_all
+
+set_option maxRecDepth 1400 in
+theorem i8_bit_and_spec {p a b}
+  : STHoare p env ⟦⟧
+    (bitAnd h![] (.i 8) h![] h![] h![a, b])
+    (fun r => r = a.and b) := by
+  resolve_trait
+  steps
+  simp_all
+
+set_option maxRecDepth 1400 in
+theorem i16_bit_and_spec {p a b}
+  : STHoare p env ⟦⟧
+    (bitAnd h![] (.i 16) h![] h![] h![a, b])
+    (fun r => r = a.and b) := by
+  resolve_trait
+  steps
+  simp_all
+
+set_option maxRecDepth 1400 in
+theorem i32_bit_and_spec {p a b}
+  : STHoare p env ⟦⟧
+    (bitAnd h![] (.i 32) h![] h![] h![a, b])
+    (fun r => r = a.and b) := by
+  resolve_trait
+  steps
+  simp_all
+
+set_option maxRecDepth 1400 in
+theorem i64_bit_and_spec {p a b}
+  : STHoare p env ⟦⟧
+    (bitAnd h![] (.i 64) h![] h![] h![a, b])
+    (fun r => r = a.and b) := by
+  resolve_trait
+  steps
+  simp_all
+
+/-- A shorthand for a call to the `std::ops::bit::BitXor::bitxor` method. -/
+@[reducible]
+def bitXor {p}
+    (generics : HList Kind.denote «std-1.0.0-beta.12::ops::bit::BitXor».«#genericKinds»)
+    (Self : Tp)
+    (associatedTypes : HList Kind.denote «std-1.0.0-beta.12::ops::bit::BitXor».«#associatedTypesKinds»)
+    (fnGenerics : HList Kind.denote «std-1.0.0-beta.12::ops::bit::BitXor».bitxor.«#genericKinds»)
+  : HList (Tp.denote p)
+      («std-1.0.0-beta.12::ops::bit::BitXor».bitxor.«#inputs» generics Self associatedTypes fnGenerics)
+  → Expr (Tp.denote p)
+      («std-1.0.0-beta.12::ops::bit::BitXor».bitxor.«#output» generics Self associatedTypes fnGenerics) :=
+  «std-1.0.0-beta.12::ops::bit::BitXor».bitxor generics Self associatedTypes fnGenerics
+
+set_option maxRecDepth 1400 in
+theorem bool_bit_xor_spec {p a b}
+  : STHoare p env ⟦⟧
+    (bitXor h![] .bool h![] h![] h![a, b])
+    (fun r => r = a.xor b) := by
+  resolve_trait
+  steps
+  simp_all
+  exact ()
+
+set_option maxRecDepth 1400 in
+theorem u128_bit_xor_spec {p a b}
+  : STHoare p env ⟦⟧
+    (bitXor h![] (.u 128) h![] h![] h![a, b])
+    (fun r => r = a.xor b) := by
+  resolve_trait
+  steps
+  simp_all
+
+set_option maxRecDepth 1400 in
+theorem u64_bit_xor_spec {p a b}
+  : STHoare p env ⟦⟧
+    (bitXor h![] (.u 64) h![] h![] h![a, b])
+    (fun r => r = a.xor b) := by
+  resolve_trait
+  steps
+  simp_all
+
+set_option maxRecDepth 1400 in
+theorem u32_bit_xor_spec {p a b}
+  : STHoare p env ⟦⟧
+    (bitXor h![] (.u 32) h![] h![] h![a, b])
+    (fun r => r = a.xor b) := by
+  resolve_trait
+  steps
+  simp_all
+
+set_option maxRecDepth 1400 in
+theorem u16_bit_xor_spec {p a b}
+  : STHoare p env ⟦⟧
+    (bitXor h![] (.u 16) h![] h![] h![a, b])
+    (fun r => r = a.xor b) := by
+  resolve_trait
+  steps
+  simp_all
+
+set_option maxRecDepth 1400 in
+theorem u8_bit_xor_spec {p a b}
+  : STHoare p env ⟦⟧
+    (bitXor h![] (.u 8) h![] h![] h![a, b])
+    (fun r => r = a.xor b) := by
+  resolve_trait
+  steps
+  simp_all
+
+set_option maxRecDepth 1450 in
+theorem u1_bit_xor_spec {p a b}
+  : STHoare p env ⟦⟧
+    (bitXor h![] (.u 1) h![] h![] h![a, b])
+    (fun r => r = a.xor b) := by
+  resolve_trait
+  steps
+  simp_all
+
+set_option maxRecDepth 1450 in
+theorem i8_bit_xor_spec {p a b}
+  : STHoare p env ⟦⟧
+    (bitXor h![] (.i 8) h![] h![] h![a, b])
+    (fun r => r = a.xor b) := by
+  resolve_trait
+  steps
+  simp_all
+
+set_option maxRecDepth 1450 in
+theorem i16_bit_xor_spec {p a b}
+  : STHoare p env ⟦⟧
+    (bitXor h![] (.i 16) h![] h![] h![a, b])
+    (fun r => r = a.xor b) := by
+  resolve_trait
+  steps
+  simp_all
+
+set_option maxRecDepth 1450 in
+theorem i32_bit_xor_spec {p a b}
+  : STHoare p env ⟦⟧
+    (bitXor h![] (.i 32) h![] h![] h![a, b])
+    (fun r => r = a.xor b) := by
+  resolve_trait
+  steps
+  simp_all
+
+set_option maxRecDepth 1450 in
+theorem i64_bit_xor_spec {p a b}
+  : STHoare p env ⟦⟧
+    (bitXor h![] (.i 64) h![] h![] h![a, b])
+    (fun r => r = a.xor b) := by
+  resolve_trait
+  steps
+  simp_all
+
+/-- A shorthand for a call to the `std::ops::bit::Shl::shl` method. -/
+@[reducible]
+def shl {p}
+    (generics : HList Kind.denote «std-1.0.0-beta.12::ops::bit::Shl».«#genericKinds»)
+    (Self : Tp)
+    (associatedTypes : HList Kind.denote «std-1.0.0-beta.12::ops::bit::Shl».«#associatedTypesKinds»)
+    (fnGenerics : HList Kind.denote «std-1.0.0-beta.12::ops::bit::Shl».shl.«#genericKinds»)
+  : HList (Tp.denote p)
+      («std-1.0.0-beta.12::ops::bit::Shl».shl.«#inputs» generics Self associatedTypes fnGenerics)
+  → Expr (Tp.denote p)
+      («std-1.0.0-beta.12::ops::bit::Shl».shl.«#output» generics Self associatedTypes fnGenerics) :=
+  «std-1.0.0-beta.12::ops::bit::Shl».shl generics Self associatedTypes fnGenerics
+
+set_option maxRecDepth 1450 in
+theorem u128_shl_spec {p a b}
+  : STHoare p env ⟦⟧
+    (shl h![] (.u 128) h![] h![] h![a, b])
+    (fun r => r = a <<< b) := by
+  resolve_trait
+  steps
+  simp_all
+
+set_option maxRecDepth 1450 in
+theorem u64_shl_spec {p a b}
+  : STHoare p env ⟦⟧
+    (shl h![] (.u 64) h![] h![] h![a, b])
+    (fun r => r = a <<< b) := by
+  resolve_trait
+  steps
+  simp_all
+
+set_option maxRecDepth 1450 in
+theorem u32_shl_spec {p a b}
+  : STHoare p env ⟦⟧
+    (shl h![] (.u 32) h![] h![] h![a, b])
+    (fun r => r = a <<< b) := by
+  resolve_trait
+  steps
+  simp_all
+
+set_option maxRecDepth 1450 in
+theorem u16_shl_spec {p a b}
+  : STHoare p env ⟦⟧
+    (shl h![] (.u 16) h![] h![] h![a, b])
+    (fun r => r = a <<< b) := by
+  resolve_trait
+  steps
+  simp_all
+
+set_option maxRecDepth 1450 in
+theorem u8_shl_spec {p a b}
+  : STHoare p env ⟦⟧
+    (shl h![] (.u 8) h![] h![] h![a, b])
+    (fun r => r = a <<< b) := by
+  resolve_trait
+  steps
+  simp_all
+
+set_option maxRecDepth 1450 in
+theorem u1_shl_spec {p a b}
+  : STHoare p env ⟦⟧
+    (shl h![] (.u 1) h![] h![] h![a, b])
+    (fun r => r = a <<< b) := by
+  resolve_trait
+  steps
+  simp_all
+
+set_option maxRecDepth 1450 in
+theorem i8_shl_spec {p a b}
+  : STHoare p env ⟦⟧
+    (shl h![] (.i 8) h![] h![] h![a, b])
+    (fun r => r = a <<< b) := by
+  resolve_trait
+  steps
+  simp_all
+
+set_option maxRecDepth 1450 in
+theorem i16_shl_spec {p a b}
+  : STHoare p env ⟦⟧
+    (shl h![] (.i 16) h![] h![] h![a, b])
+    (fun r => r = a <<< b) := by
+  resolve_trait
+  steps
+  simp_all
+
+set_option maxRecDepth 1450 in
+theorem i32_shl_spec {p a b}
+  : STHoare p env ⟦⟧
+    (shl h![] (.i 32) h![] h![] h![a, b])
+    (fun r => r = a <<< b) := by
+  resolve_trait
+  steps
+  simp_all
+
+set_option maxRecDepth 1450 in
+theorem i64_shl_spec {p a b}
+  : STHoare p env ⟦⟧
+    (shl h![] (.i 64) h![] h![] h![a, b])
+    (fun r => r = a <<< b) := by
+  resolve_trait
+  steps
+  simp_all
+
+/-- A shorthand for a call to the `std::ops::bit::Shr::shr` method. -/
+@[reducible]
+def shr {p}
+    (generics : HList Kind.denote «std-1.0.0-beta.12::ops::bit::Shr».«#genericKinds»)
+    (Self : Tp)
+    (associatedTypes : HList Kind.denote «std-1.0.0-beta.12::ops::bit::Shr».«#associatedTypesKinds»)
+    (fnGenerics : HList Kind.denote «std-1.0.0-beta.12::ops::bit::Shr».shr.«#genericKinds»)
+  : HList (Tp.denote p)
+      («std-1.0.0-beta.12::ops::bit::Shr».shr.«#inputs» generics Self associatedTypes fnGenerics)
+  → Expr (Tp.denote p)
+      («std-1.0.0-beta.12::ops::bit::Shr».shr.«#output» generics Self associatedTypes fnGenerics) :=
+  «std-1.0.0-beta.12::ops::bit::Shr».shr generics Self associatedTypes fnGenerics
+
+set_option maxRecDepth 1450 in
+theorem u128_shr_spec {p a b}
+  : STHoare p env ⟦⟧
+    (shr h![] (.u 128) h![] h![] h![a, b])
+    (fun r => r = a >>> b) := by
+  resolve_trait
+  steps
+  simp_all
+
+set_option maxRecDepth 1450 in
+theorem u64_shr_spec {p a b}
+  : STHoare p env ⟦⟧
+    (shr h![] (.u 64) h![] h![] h![a, b])
+    (fun r => r = a >>> b) := by
+  resolve_trait
+  steps
+  simp_all
+
+set_option maxRecDepth 1500 in
+theorem u32_shr_spec {p a b}
+  : STHoare p env ⟦⟧
+    (shr h![] (.u 32) h![] h![] h![a, b])
+    (fun r => r = a >>> b) := by
+  resolve_trait
+  steps
+  simp_all
+
+set_option maxRecDepth 1500 in
+theorem u16_shr_spec {p a b}
+  : STHoare p env ⟦⟧
+    (shr h![] (.u 16) h![] h![] h![a, b])
+    (fun r => r = a >>> b) := by
+  resolve_trait
+  steps
+  simp_all
+
+set_option maxRecDepth 1500 in
+theorem u8_shr_spec {p a b}
+  : STHoare p env ⟦⟧
+    (shr h![] (.u 8) h![] h![] h![a, b])
+    (fun r => r = a >>> b) := by
+  resolve_trait
+  steps
+  simp_all
+
+set_option maxRecDepth 1500 in
+theorem u1_shr_spec {p a b}
+  : STHoare p env ⟦⟧
+    (shr h![] (.u 1) h![] h![] h![a, b])
+    (fun r => r = a >>> b) := by
+  resolve_trait
+  steps
+  simp_all
+
+set_option maxRecDepth 1500 in
+theorem i8_shr_spec {p a b}
+  : STHoare p env ⟦⟧
+    (shr h![] (.i 8) h![] h![] h![a, b])
+    (fun r => r = a >>> b) := by
+  resolve_trait
+  steps
+  simp_all
+
+set_option maxRecDepth 1500 in
+theorem i16_shr_spec {p a b}
+  : STHoare p env ⟦⟧
+    (shr h![] (.i 16) h![] h![] h![a, b])
+    (fun r => r = a >>> b) := by
+  resolve_trait
+  steps
+  simp_all
+
+set_option maxRecDepth 1500 in
+theorem i32_shr_spec {p a b}
+  : STHoare p env ⟦⟧
+    (shr h![] (.i 32) h![] h![] h![a, b])
+    (fun r => r = a >>> b) := by
+  resolve_trait
+  steps
+  simp_all
+
+set_option maxRecDepth 1500 in
+theorem i64_shr_spec {p a b}
+  : STHoare p env ⟦⟧
+    (shr h![] (.i 64) h![] h![] h![a, b])
+    (fun r => r = a >>> b) := by
+  resolve_trait
+  steps
+  simp_all
+
