stdlib/lampe/Stdlib/Lib.lean
@@ -4,3 +4,4 @@ import Lampe
 namespace Lampe.Stdlib.Lib
 
 open «std-1.0.0-beta.12»
+
