stdlib/lampe/Stdlib/Stdlib.lean
@@ -34,3 +34,4 @@ import «std-1.0.0-beta.12».Extracted
 namespace Lampe.Stdlib
 
 export «std-1.0.0-beta.12» (env)
+
