stdlib/lampe/Stdlib/Tp.lean
@@ -6,3 +6,4 @@ set_option Lampe.pp.Expr false
 set_option Lampe.pp.STHoare false
 
 abbrev comparator (p : Prime) (t : Tp) : Type := t.denote p → t.denote p → Ordering
+
